ssl-spawning-displacement-proof/proofs/GeneratedClightFacts.v
@@ -1,6 +1,8 @@
-From Coq Require Import List PArith.BinPos String.
+From Coq Require Import List PArith.BinPos String ZArith.
 From compcert Require Import AST Clight Clightdefs.
 From SSLSpawning.Generated Require Import
+  jp_area jp_level_update jp_level_script jp_ssl_script
+  jp_ssl_area1_macro jp_ssl_area2_macro jp_behavior_data
   jp_object_list_processor jp_platform_displacement jp_spawn_object
   jp_obj_behaviors.
 From SSLSpawning.Proofs Require Import ASTFacts.
@@ -14,6 +16,13 @@ Module O := jp_object_list_processor.
 Module P := jp_platform_displacement.
 Module S := jp_spawn_object.
 Module B := jp_obj_behaviors.
+Module A := jp_area.
+Module L := jp_level_update.
+Module LS := jp_level_script.
+Module SSL := jp_ssl_script.
+Module M1 := jp_ssl_area1_macro.
+Module M2 := jp_ssl_area2_macro.
+Module BD := jp_behavior_data.
 
 Definition id_clear_mario_platform : ident := $"clear_mario_platform".
 
@@ -74,6 +83,68 @@ Proof.
   reflexivity.
 Qed.
 
+Theorem generated_update_mario_platform_calls_find_floor :
+  calls_ident_s P._find_floor
+    (fn_body P.f_update_mario_platform) = true.
+Proof.
+  vm_compute.
+  reflexivity.
+Qed.
+
+Theorem generated_update_mario_platform_reads_floor_object :
+  statement_mentions_ident_s P._object
+    (fn_body P.f_update_mario_platform) = true.
+Proof.
+  vm_compute.
+  reflexivity.
+Qed.
+
+Theorem generated_update_mario_platform_writes_gMarioPlatform :
+  statement_mentions_ident_s P._gMarioPlatform
+    (fn_body P.f_update_mario_platform) = true.
+Proof.
+  vm_compute.
+  reflexivity.
+Qed.
+
+Theorem generated_update_mario_platform_writes_mario_object_platform :
+  assigns_field_named_s P._platform
+    (fn_body P.f_update_mario_platform) = true.
+Proof.
+  vm_compute.
+  reflexivity.
+Qed.
+
+Theorem generated_apply_platform_displacement_uses_raw_object_slots :
+  statement_mentions_ident_s P._rawData
+    (fn_body P.f_apply_platform_displacement) = true /\
+  statement_mentions_ident_s P._asF32
+    (fn_body P.f_apply_platform_displacement) = true /\
+  statement_mentions_ident_s P._asS32
+    (fn_body P.f_apply_platform_displacement) = true /\
+  statement_mentions_int_s 9
+    (fn_body P.f_apply_platform_displacement) = true /\
+  statement_mentions_int_s 11
+    (fn_body P.f_apply_platform_displacement) = true /\
+  statement_mentions_int_s 35
+    (fn_body P.f_apply_platform_displacement) = true /\
+  statement_mentions_int_s 36
+    (fn_body P.f_apply_platform_displacement) = true /\
+  statement_mentions_int_s 37
+    (fn_body P.f_apply_platform_displacement) = true.
+Proof.
+  vm_compute.
+  repeat split.
+Qed.
+
+Theorem generated_apply_platform_displacement_updates_mario_position :
+  calls_ident_s P._set_mario_pos
+    (fn_body P.f_apply_platform_displacement) = true.
+Proof.
+  vm_compute.
+  reflexivity.
+Qed.
+
 Theorem generated_update_objects_call_order :
   ident_subsequenceb
     [O._clear_dynamic_surfaces;
@@ -119,4 +190,265 @@ Theorem generated_obj_behaviors_contains_spindel_loop :
 Proof.
   vm_compute.
   reflexivity.
+Qed.
+
+Theorem generated_spindel_loop_mentions_velocity_and_pitch_slots :
+  statement_mentions_ident_s B._rawData
+    (fn_body B.f_bhv_spindel_loop) = true /\
+  statement_mentions_ident_s B._asF32
+    (fn_body B.f_bhv_spindel_loop) = true /\
+  statement_mentions_ident_s B._asS32
+    (fn_body B.f_bhv_spindel_loop) = true /\
+  statement_mentions_int_s 11
+    (fn_body B.f_bhv_spindel_loop) = true /\
+  statement_mentions_int_s 35
+    (fn_body B.f_bhv_spindel_loop) = true /\
+  statement_mentions_int_s 1024
+    (fn_body B.f_bhv_spindel_loop) = true.
+Proof.
+  vm_compute.
+  repeat split.
+Qed.
+
+Theorem generated_load_area_calls_spawn_objects_from_info :
+  calls_ident_s A._spawn_objects_from_info
+    (fn_body A.f_load_area) = true.
+Proof.
+  vm_compute.
+  reflexivity.
+Qed.
+
+Theorem generated_load_mario_area_calls_spawn_objects_from_info :
+  calls_ident_s A._spawn_objects_from_info
+    (fn_body A.f_load_mario_area) = true.
+Proof.
+  vm_compute.
+  reflexivity.
+Qed.
+
+Theorem generated_level_cmd_init_level_calls_clear_objects :
+  calls_ident_s LS._clear_objects
+    (fn_body LS.f_level_cmd_init_level) = true.
+Proof.
+  vm_compute.
+  reflexivity.
+Qed.
+
+Theorem generated_play_mode_normal_updates_objects_before_painting_warp :
+  ident_subsequenceb
+    [L._area_update_objects; L._initiate_painting_warp]
+    (direct_callees_s (fn_body L.f_play_mode_normal)) = true.
+Proof.
+  vm_compute.
+  reflexivity.
+Qed.
+
+Theorem generated_initiate_painting_warp_uses_checkpoint_then_warp :
+  calls_ident_s L._check_warp_checkpoint
+    (fn_body L.f_initiate_painting_warp) = true /\
+  calls_ident_s L._initiate_warp
+    (fn_body L.f_initiate_painting_warp) = true.
+Proof.
+  vm_compute.
+  repeat split.
+Qed.
+
+Theorem generated_get_painting_warp_node_reads_floor_type :
+  statement_mentions_ident_s L._floor
+    (fn_body L.f_get_painting_warp_node) = true /\
+  statement_mentions_ident_s L._type
+    (fn_body L.f_get_painting_warp_node) = true.
+Proof.
+  vm_compute.
+  repeat split.
+Qed.
+
+Theorem generated_ssl_area2_macro_object_count_is_50 :
+  ((List.length (gvar_init M2.v_ssl_seg7_area_2_macro_objs) - 1) / 5)%nat =
+    50%nat.
+Proof.
+  vm_compute.
+  reflexivity.
+Qed.
+
+Theorem generated_ssl_area1_macro_object_count_is_46 :
+  ((List.length (gvar_init M1.v_ssl_seg7_area_1_macro_objs) - 1) / 5)%nat =
+    46%nat.
+Proof.
+  vm_compute.
+  reflexivity.
+Qed.
+
+Theorem generated_ssl_area2_regular_script_has_spindel_targets :
+  initializer_list_mentions_addrof SSL._bhvSpindel
+    (gvar_init SSL.v_script_func_local_4) = true /\
+  initializer_list_mentions_addrof SSL._bhvPyramidElevator
+    (gvar_init SSL.v_script_func_local_4) = true /\
+  initializer_list_mentions_addrof SSL._bhvSSLMovingPyramidWall
+    (gvar_init SSL.v_script_func_local_4) = true /\
+  initializer_list_mentions_addrof SSL._bhvGrindel
+    (gvar_init SSL.v_script_func_local_4) = true /\
+  initializer_list_mentions_addrof SSL._bhvHorizontalGrindel
+    (gvar_init SSL.v_script_func_local_4) = true.
+Proof.
+  vm_compute.
+  repeat split.
+Qed.
+
+Theorem generated_ssl_area2_regular_script_spindel_precedes_elevator_source_order :
+  ident_subsequenceb
+    [SSL._bhvSpindel; SSL._bhvSSLMovingPyramidWall; SSL._bhvPyramidElevator]
+    (initializer_addrofs (gvar_init SSL.v_script_func_local_4)) = true.
+Proof.
+  vm_compute.
+  reflexivity.
+Qed.
+
+Theorem generated_ssl_area1_regular_script_has_seed_platforms :
+  initializer_list_mentions_addrof SSL._bhvPyramidTop
+    (gvar_init SSL.v_script_func_local_1) = true /\
+  initializer_list_mentions_addrof SSL._bhvToxBox
+    (gvar_init SSL.v_script_func_local_2) = true.
+Proof.
+  vm_compute.
+  repeat split.
+Qed.
+
+Theorem generated_ssl_level_entry_has_area_warps :
+  initializer_list_mentions_addrof SSL._bhvWarp
+    (gvar_init SSL.v_level_ssl_entry) = true.
+Proof.
+  vm_compute.
+  reflexivity.
+Qed.
+
+Theorem generated_bhv_spindel_loads_collision_and_loop :
+  initializer_list_mentions_addrof BD._ssl_seg7_collision_spindel
+    (gvar_init BD.v_bhvSpindel) = true /\
+  initializer_list_mentions_addrof BD._bhv_spindel_loop
+    (gvar_init BD.v_bhvSpindel) = true /\
+  initializer_list_mentions_addrof BD._load_object_collision_model
+    (gvar_init BD.v_bhvSpindel) = true.
+Proof.
+  vm_compute.
+  repeat split.
+Qed.
+
+Theorem generated_bhv_exclamation_box_has_collision_and_loop :
+  initializer_list_mentions_addrof BD._exclamation_box_outline_seg8_collision_08025F78
+    (gvar_init BD.v_bhvExclamationBox) = true /\
+  initializer_list_mentions_addrof BD._bhv_exclamation_box_loop
+    (gvar_init BD.v_bhvExclamationBox) = true.
+Proof.
+  vm_compute.
+  repeat split.
+Qed.
+
+Theorem generated_bhv_carry_something_behaviors_do_not_load_collision :
+  initializer_list_mentions_addrof BD._load_object_collision_model
+    (gvar_init BD.v_bhvCarrySomething3) = false /\
+  initializer_list_mentions_addrof BD._load_object_collision_model
+    (gvar_init BD.v_bhvCarrySomething4) = false.
+Proof.
+  vm_compute.
+  repeat split.
+Qed.
+
+Theorem generated_bhv_pyramid_top_and_tox_box_name_collision_data :
+  initializer_list_mentions_addrof BD._ssl_seg7_collision_pyramid_top
+    (gvar_init BD.v_bhvPyramidTop) = true /\
+  initializer_list_mentions_addrof BD._load_object_collision_model
+    (gvar_init BD.v_bhvPyramidTop) = true /\
+  initializer_list_mentions_addrof BD._ssl_seg7_collision_tox_box
+    (gvar_init BD.v_bhvToxBox) = true /\
+  initializer_list_mentions_addrof BD._bhv_tox_box_loop
+    (gvar_init BD.v_bhvToxBox) = true.
+Proof.
+  vm_compute.
+  repeat split.
+Qed.
+
+Theorem generated_behavior_globals_are_linked_in_behavior_data :
+  program_global_initializer BD.prog BD._bhvSpindel =
+    Some (gvar_init BD.v_bhvSpindel) /\
+  program_global_initializer BD.prog BD._bhvExclamationBox =
+    Some (gvar_init BD.v_bhvExclamationBox) /\
+  program_global_initializer BD.prog BD._bhvPyramidTop =
+    Some (gvar_init BD.v_bhvPyramidTop) /\
+  program_global_initializer BD.prog BD._bhvToxBox =
+    Some (gvar_init BD.v_bhvToxBox).
+Proof.
+  vm_compute.
+  repeat split.
+Qed.
+
+Record jp_clight_source_certificate : Prop := {
+  cert_spawn_no_clear :
+    calls_ident_s id_clear_mario_platform
+      (fn_body O.f_spawn_objects_from_info) = false;
+  cert_apply_reads_platform :
+    statement_mentions_ident_s P._gMarioPlatform
+      (fn_body P.f_apply_mario_platform_displacement) = true;
+  cert_apply_calls_platform_displacement :
+    calls_ident_s P._apply_platform_displacement
+      (fn_body P.f_apply_mario_platform_displacement) = true;
+  cert_apply_no_active_check :
+    statement_mentions_ident_s P._activeFlags
+      (fn_body P.f_apply_mario_platform_displacement) = false;
+  cert_apply_no_behavior_check :
+    statement_mentions_ident_s P._behavior
+      (fn_body P.f_apply_mario_platform_displacement) = false;
+  cert_apply_no_collision_check :
+    statement_mentions_ident_s P._collisionData
+      (fn_body P.f_apply_mario_platform_displacement) = false;
+  cert_update_mario_platform_floor_object :
+    statement_mentions_ident_s P._object
+      (fn_body P.f_update_mario_platform) = true;
+  cert_update_order :
+    ident_subsequenceb
+      [O._clear_dynamic_surfaces;
+       O._update_terrain_objects;
+       O._apply_mario_platform_displacement;
+       O._detect_object_collisions;
+       O._update_non_terrain_objects;
+       O._unload_deactivated_objects;
+       O._update_mario_platform]
+      (direct_callees_s (fn_body O.f_update_objects)) = true;
+  cert_unload_deallocates :
+    calls_ident_s S._deallocate_object (fn_body S.f_unload_object) = true;
+  cert_allocate_pops_next :
+    assigns_field_named_s S._next
+      (fn_body S.f_try_allocate_object) = true;
+  cert_area2_macro_count :
+    ((List.length (gvar_init M2.v_ssl_seg7_area_2_macro_objs) - 1) / 5)%nat =
+      50%nat;
+  cert_area2_script_has_spindel :
+    initializer_list_mentions_addrof SSL._bhvSpindel
+      (gvar_init SSL.v_script_func_local_4) = true;
+  cert_spindel_behavior_loads_collision_and_loop :
+    initializer_list_mentions_addrof BD._ssl_seg7_collision_spindel
+      (gvar_init BD.v_bhvSpindel) = true /\
+    initializer_list_mentions_addrof BD._bhv_spindel_loop
+      (gvar_init BD.v_bhvSpindel) = true /\
+    initializer_list_mentions_addrof BD._load_object_collision_model
+      (gvar_init BD.v_bhvSpindel) = true;
+  cert_spindel_loop_raw_slots :
+    statement_mentions_ident_s B._rawData
+      (fn_body B.f_bhv_spindel_loop) = true /\
+    statement_mentions_ident_s B._asF32
+      (fn_body B.f_bhv_spindel_loop) = true /\
+    statement_mentions_ident_s B._asS32
+      (fn_body B.f_bhv_spindel_loop) = true /\
+    statement_mentions_int_s 11
+      (fn_body B.f_bhv_spindel_loop) = true /\
+    statement_mentions_int_s 35
+      (fn_body B.f_bhv_spindel_loop) = true /\
+    statement_mentions_int_s 1024
+      (fn_body B.f_bhv_spindel_loop) = true
+}.
+
+Theorem generated_jp_clight_source_certificate :
+  jp_clight_source_certificate.
+Proof.
+  constructor; vm_compute; repeat split.
 Qed.
